refactoring substitutions and manipulations.
- full proofs in RTac/Ctx.

theories/ExprI.v
@@ -154,11 +154,21 @@ Section Expr.
                          option (exprT us vs (typD t))
   ; Expr_acc : relation expr
   ; wf_Expr_acc : well_founded Expr_acc
-    (** This is derivable from information in variables, it is also
-     ** bad for reasoning about
-     **)
-(*  ; mentionsAny : (uvar -> bool) -> (var -> bool) -> expr -> bool *)
+  ; mentionsAny : (uvar -> bool) -> (var -> bool) -> expr -> bool
+  ; mentionsU : uvar -> expr -> bool
+  ; mentionsV : var -> expr -> bool
+  ; expr_subst
+    : (uvar -> option expr) -> (var -> option expr) -> nat -> expr -> expr
   }.
+
+  Definition exprD {E : Expr} (uvar_env var_env : env) (e : expr) (t : typ)
+  : option (typD t) :=
+    let (tus,us) := split_env uvar_env in
+    let (tvs,vs) := split_env var_env in
+    match exprD' tus tvs e t with
+      | None => None
+      | Some f => Some (f us vs)
+    end.
 
   Theorem exprD'_conv (E : Expr)
   : forall tus tus' tvs tvs' e t
@@ -173,33 +183,89 @@ Section Expr.
     destruct pfu. destruct pfv. reflexivity.
   Qed.
 
-  Definition Safe_expr {E : Expr} (tus tvs : tenv typ) (e : expr) (t : typ)
+  Record ExprTApplicativeR (tus tvs tus' tvs' : tenv typ)
+         (C : exprT tus tvs (exprT tus' tvs' Prop) -> Prop)
+  : Type :=
+  { exprTPureR : forall (P : exprT tus tvs (exprT tus' tvs' Prop)),
+      (forall a b c d, P a b c d) -> C P
+  ; exprTApR : forall P Q : exprT tus tvs (exprT tus' tvs' Prop),
+        C (fun a b c d => P a b c d -> Q a b c d) -> C P -> C Q
+  }.
+
+  Definition expr_subst_spec_ho
+             (exprD' : forall (us vs : tenv typ),
+               expr -> forall (t : typ),
+                         option (exprT us vs (typD t)))
+             (expr_subst : (uvar -> option expr) -> (var -> option expr) -> nat -> expr -> expr)
   : Prop :=
-    exists val, exprD' tus tvs e t = Some val.
+    forall substU substV n e e',
+      expr_subst substU substV n e = e' ->
+      forall _tvs tus tvs tus' tvs'
+             (P : exprT tus tvs (exprT tus' tvs' Prop) -> Prop)
+             (ExprTApR : ExprTApplicativeR P)
+             (H_substU : forall u t get,
+                 nth_error_get_hlist_nth typD tus u = Some (@existT _ _ t get) ->
+                 match substU u with
+                   | Some eU =>
+                     exists eUD,
+                     exprD' tus' tvs' eU t = Some eUD /\
+                     P (fun us vs us' vs' => get us = eUD us' vs')
+                   | None => exists get',
+                             nth_error_get_hlist_nth typD tus' u = Some (@existT _ _ t get')
+                             /\ P (fun us vs us' vs' => get us = get' us')
+                 end)
+             (H_substV : forall u t get,
+                 nth_error_get_hlist_nth typD tvs u = Some (@existT _ _ t get) ->
+                 match substV u with
+                   | Some eV =>
+                     exists eVD,
+                     exprD' tus' tvs' eV t = Some eVD /\
+                     P (fun us vs us' vs' => get vs = eVD us' vs')
+                   | None => exists get',
+                             nth_error_get_hlist_nth typD tvs' u = Some (@existT _ _ t get')
+                             /\ P (fun us vs us' vs' => get vs = get' vs')
+                 end),
+      forall t eD,
+        length _tvs = n ->
+        exprD' tus (_tvs ++ tvs) e t = Some eD ->
+        exists eD',
+          exprD' tus' (_tvs ++ tvs') e' t = Some eD' /\
+          P (fun us vs us' vs' => forall _vs,
+                 eD us (HList.hlist_app _vs vs) = eD' us' (HList.hlist_app _vs vs')).
 
-  Theorem Safe_expr_exprD {E : Expr}
-  : forall us vs e t,
-      Safe_expr us vs e t <->
-      exists val, exprD' us vs e t = Some val.
-  Proof. reflexivity. Qed.
+  Definition mentionsU_subst_spec
+             (expr_subst : (uvar -> option expr) -> (var -> option expr) -> nat -> expr -> expr)
+             (mentionsU : uvar -> expr -> bool)
+             (mentionsV : var -> expr -> bool)
+  : Prop :=
+    forall substU substV n u e,
+      mentionsU u (expr_subst substU substV n e) = true <->
+      (   (mentionsU u e = true /\ substU u = None)
+       \/ (exists u' e', mentionsU u' e = true /\
+                         substU u' = Some e' /\
+                         mentionsU u e' = true)
+       \/ (exists v' e', mentionsV (n+v') e = true /\
+                         substV v' = Some e' /\
+                         mentionsU u e' = true)).
 
-  Definition exprD {E : Expr} (uvar_env var_env : env) (e : expr) (t : typ)
-  : option (typD t) :=
-    let (tus,us) := split_env uvar_env in
-    let (tvs,vs) := split_env var_env in
-    match exprD' tus tvs e t with
-      | None => None
-      | Some f => Some (f us vs)
-    end.
+  Definition mentionsV_subst_spec
+             (expr_subst : (uvar -> option expr) -> (var -> option expr) -> nat -> expr -> expr)
+             (mentionsU : uvar -> expr -> bool)
+             (mentionsV : var -> expr -> bool)
+  : Prop :=
+    forall substU substV n v e,
+      mentionsV v (expr_subst substU substV n e) = true <->
+      (   (v < n /\ mentionsV v e = true)
+       \/ (v >= n /\
+           (   (mentionsV v e = true /\ substV (v-n) = None)
+            \/ (exists u' e', mentionsU u' e = true /\
+                              substU u' = Some e' /\
+                              mentionsV (v-n) e' = true)
+            \/ (exists v' e', mentionsV (v'+n) e = true /\
+                              substV v' = Some e' /\
+                              mentionsV (v-n) e' = true)))).
 
-(*
-  Definition mentionsV {Expr : Expr} (v : var) (e : expr) : bool :=
-    mentionsAny (fun _ => false) (fun v' => v ?[ eq ] v') e.
-  Definition mentionsU {Expr : Expr} (u : uvar) (e : expr) : bool :=
-    mentionsAny (fun u' => u ?[ eq ] u') (fun _ => false) e.
-*)
-
-  Class ExprOk (E : Expr) : Type :=
+  Class ExprOk (E : Expr) : Prop :=
   { exprD'_weaken
     : forall tus tvs e t val,
         exprD' tus tvs e t = Some val ->
@@ -208,8 +274,6 @@ Section Expr.
              exprD' (tus ++ tus') (tvs ++ tvs') e t = Some val'
           /\ forall us vs us' vs',
                val us vs = val' (hlist_app us us') (hlist_app vs vs')
-    (** TODO: These are in Variables **)
-(*
   ; exprD'_strengthenU_single
     : forall tus tvs e t t' val,
       mentionsU (length tus) e = false ->
@@ -228,16 +292,106 @@ Section Expr.
           val us (hlist_app vs (Hcons u Hnil)) = val' us vs
   ; Proper_mentionsAny
     : Proper ((eq ==> eq) ==> (eq ==> eq) ==> eq ==> eq) mentionsAny
+  ; mentionsAny_weaken_strong
+    : forall pu pu' pv pv' e,
+        (forall u, mentionsU u e = true -> pu u = false -> pu' u = false) ->
+        (forall v, mentionsV v e = true -> pv v = false -> pv' v = false) ->
+        mentionsAny pu pv e = false ->
+        mentionsAny pu' pv' e = false
   ; mentionsAny_factor
     : forall fu fu' fv fv' e,
           mentionsAny (fun u => fu u || fu' u) (fun v => fv v || fv' v) e
         = mentionsAny fu fv e || mentionsAny fu' fv' e
-*)
+  ; mentionsAny_complete
+    : forall pu pv e,
+        mentionsAny pu pv e = true <->
+        (exists u, mentionsU u e = true /\ pu u = true) \/
+        (exists v, mentionsV v e = true /\ pv v = true)
+  ; mentionsAny_mentionsU
+    : forall u e,
+        mentionsU u e = mentionsAny (fun u' => u ?[ eq ] u') (fun _ => false) e
+  ; mentionsAny_mentionsV
+    : forall u e,
+        mentionsV u e = mentionsAny (fun _ => false) (fun u' => u ?[ eq ] u') e
+  ; expr_subst_sound_ho
+    : forall substU substV n e e',
+      expr_subst substU substV n e = e' ->
+      forall _tvs tus tvs tus' tvs'
+             (P : exprT tus tvs (exprT tus' tvs' Prop) -> Prop)
+             (ExprTApR : ExprTApplicativeR P)
+             (H_substU : forall u t get,
+                 nth_error_get_hlist_nth typD tus u = Some (@existT _ _ t get) ->
+                 match substU u with
+                   | Some eU =>
+                     exists eUD,
+                     exprD' tus' tvs' eU t = Some eUD /\
+                     P (fun us vs us' vs' => get us = eUD us' vs')
+                   | None => exists get',
+                             nth_error_get_hlist_nth typD tus' u = Some (@existT _ _ t get')
+                             /\ P (fun us vs us' vs' => get us = get' us')
+                 end)
+             (H_substV : forall u t get,
+                 nth_error_get_hlist_nth typD tvs u = Some (@existT _ _ t get) ->
+                 match substV u with
+                   | Some eV =>
+                     exists eVD,
+                     exprD' tus' tvs' eV t = Some eVD /\
+                     P (fun us vs us' vs' => get vs = eVD us' vs')
+                   | None => exists get',
+                             nth_error_get_hlist_nth typD tvs' u = Some (@existT _ _ t get')
+                             /\ P (fun us vs us' vs' => get vs = get' vs')
+                 end),
+      forall t eD,
+        length _tvs = n ->
+        exprD' tus (_tvs ++ tvs) e t = Some eD ->
+        exists eD',
+          exprD' tus' (_tvs ++ tvs') e' t = Some eD' /\
+          P (fun us vs us' vs' => forall _vs,
+                 eD us (HList.hlist_app _vs vs) = eD' us' (HList.hlist_app _vs vs'))
+  ; expr_subst_noop : forall substU substV n e,
+      (forall u, mentionsU u e = true -> substU u = None) ->
+      (forall v, mentionsV (v+n) e = true -> substV v = None) ->
+      expr_subst substU substV n e = e
+  ; mentionsU_subst
+    : forall substU substV n u e,
+      mentionsU u (expr_subst substU substV n e) = true <->
+      (   (mentionsU u e = true /\ substU u = None)
+       \/ (exists u' e', mentionsU u' e = true /\
+                         substU u' = Some e' /\
+                         mentionsU u e' = true)
+       \/ (exists v' e', mentionsV (n+v') e = true /\
+                         substV v' = Some e' /\
+                         mentionsU u e' = true))
+  ; mentionsV_subst
+    : forall substU substV n v e,
+      mentionsV v (expr_subst substU substV n e) = true <->
+      (   (v < n /\ mentionsV v e = true)
+       \/ (v >= n /\
+           (   (mentionsV v e = true /\ substV (v-n) = None)
+            \/ (exists u' e', mentionsU u' e = true /\
+                              substU u' = Some e' /\
+                              mentionsV (v-n) e' = true)
+            \/ (exists v' e', mentionsV (v'+n) e = true /\
+                              substV v' = Some e' /\
+                              mentionsV (v-n) e' = true))))
+  ; Proper_subst
+    : Proper ((eq ==> eq) ==> (eq ==> eq) ==> eq ==> eq ==> eq) expr_subst
   }.
 
   Context {Expr_expr : Expr}.
+  Context {ExprOk_expr : ExprOk Expr_expr}.
 
-  Lemma exprD'_weakenU (EOk : ExprOk Expr_expr)
+  Theorem mentionsAny_weaken
+  : forall pu pu' pv pv',
+      (forall u, pu u = false -> pu' u = false) ->
+      (forall v, pv v = false -> pv' v = false) ->
+      forall e, mentionsAny pu pv e = false ->
+                mentionsAny pu' pv' e = false.
+  Proof.
+    intros. revert H1. eapply mentionsAny_weaken_strong; eauto.
+  Qed.
+
+  Lemma exprD'_weakenU
   : forall tus tus' tvs e t val,
       exprD' tus tvs e t = Some val ->
       exists val',
@@ -270,7 +424,7 @@ Section Expr.
       reflexivity. }
   Qed.
 
-  Lemma exprD'_weakenV (EOk : ExprOk Expr_expr)
+  Lemma exprD'_weakenV
   : forall tus tvs tvs' e t val,
       exprD' tus tvs e t = Some val ->
       exists val',
@@ -303,7 +457,7 @@ Section Expr.
       reflexivity. }
   Qed.
 
-  Theorem exprD_weaken (EOk : ExprOk Expr_expr)
+  Theorem exprD_weaken
   : forall us us' vs vs' e t val,
       exprD us vs e t = Some val ->
       exprD (us ++ us') (vs ++ vs') e t = Some val.
@@ -319,6 +473,7 @@ Section Expr.
     rewrite H. rewrite <- H0. reflexivity.
   Qed.
 
+  (** TODO: Move to ExtLib.Data.List. **)
   Lemma list_rev_ind
   : forall T (P : list T -> Prop),
       P nil ->
@@ -331,12 +486,185 @@ Section Expr.
     simpl. auto.
   Qed.
 
-(*
-*)
+  Theorem exprD'_strengthenV_multi
+  : forall tus tvs e  t' tvs' val,
+      (forall v, v < length tvs' ->
+                 mentionsV (length tvs + v) e = false) ->
+      exprD' tus (tvs ++ tvs') e t' = Some val ->
+      exists val',
+        exprD' tus tvs e t' = Some val' /\
+        forall us vs vs',
+          val us (hlist_app vs vs') = val' us vs.
+  Proof.
+    intros tus tvs e t'.
+    refine (@list_rev_ind _ _ _ _).
+    { simpl. intros.
+      rewrite exprD'_conv with (pfv := app_nil_r_trans tvs) (pfu := eq_refl).
+      rewrite H0. autorewrite with eq_rw.
+      eexists; split; eauto.
+      intros. rewrite (hlist_eta vs').
+      rewrite hlist_app_nil_r.
+      reflexivity. }
+    { intros.
+      rewrite exprD'_conv with (pfv := app_ass_trans tvs ls (l :: nil))
+                               (pfu := eq_refl) in H1.
+      autorewrite with eq_rw in H1.
+      forward.
+      eapply exprD'_strengthenV_single in H1.
+      + forward_reason.
+        eapply H in H1.
+        - forward_reason.
+          eexists; split; eauto.
+          intros. inv_all; subst.
+          clear - H3 H4.
+          specialize (H4 us vs (fst (hlist_split _ _ vs'))).
+          specialize (H3 us (hlist_app vs (fst (hlist_split _ _ vs')))
+                         (hlist_hd (snd (hlist_split _ _ vs')))).
+          rewrite <- H4; clear H4.
+          rewrite <- H3; clear H3.
+          autorewrite with eq_rw.
+          f_equal.
+          rewrite hlist_app_assoc.
+          apply match_eq_match_eq.
+          f_equal.
+          etransitivity.
+          symmetry.
+          eapply (hlist_app_hlist_split _ _ vs').
+          f_equal.
+          rewrite (hlist_eta (snd (hlist_split _ _ _))).
+          simpl. f_equal.
+          rewrite (hlist_eta (hlist_tl _)). reflexivity.
+        - intros.
+          eapply H0. rewrite app_length. simpl. omega.
+      + rewrite app_length.
+        apply H0. rewrite app_length. simpl. omega. }
+  Qed.
+
+  Theorem exprD'_strengthenU_multi
+  : forall tus tvs e  t' tus' val,
+      (forall u, u < length tus' ->
+                 mentionsU (length tus + u) e = false) ->
+      exprD' (tus ++ tus') tvs e t' = Some val ->
+      exists val',
+        exprD' tus tvs e t' = Some val' /\
+        forall us vs us',
+          val (hlist_app us us') vs = val' us vs.
+  Proof.
+    intros tus tvs e t'.
+    refine (@list_rev_ind _ _ _ _).
+    { simpl. intros.
+      rewrite exprD'_conv with (pfu := app_nil_r_trans tus) (pfv := eq_refl).
+      rewrite H0. autorewrite with eq_rw.
+      eexists; split; eauto.
+      intros. rewrite (hlist_eta us').
+      rewrite hlist_app_nil_r. reflexivity. }
+    { intros.
+      rewrite exprD'_conv with (pfu := app_ass_trans tus ls (l :: nil)) (pfv := eq_refl) in H1.
+      autorewrite with eq_rw in H1.
+      forward.
+      eapply exprD'_strengthenU_single in H1.
+      + forward_reason.
+        eapply H in H1.
+        - forward_reason.
+          eexists; split; eauto.
+          intros. inv_all; subst.
+          clear - H3 H4.
+          specialize (H4 us vs (fst (hlist_split _ _ us'))).
+          specialize (H3 (hlist_app us (fst (hlist_split _ _ us')))
+                         vs (hlist_hd (snd (hlist_split _ _ us')))).
+          rewrite <- H4; clear H4.
+          rewrite <- H3; clear H3.
+          repeat rewrite eq_Arr_eq. repeat rewrite eq_Const_eq.
+          f_equal.
+          rewrite hlist_app_assoc.
+          autorewrite with eq_rw.
+          f_equal.
+          eapply match_eq_match_eq.
+          f_equal.
+          etransitivity. symmetry. eapply (hlist_app_hlist_split _ _ us').
+          f_equal.
+          rewrite (hlist_eta (snd (hlist_split _ _ _))).
+          simpl. f_equal.
+          rewrite (hlist_eta (hlist_tl _)). reflexivity.
+        - intros.
+          eapply H0. rewrite app_length. simpl. omega.
+      + rewrite app_length.
+        apply H0. rewrite app_length. simpl. omega. }
+  Qed.
+
+  Theorem expr_subst_sound
+  : forall substU substV n e e',
+      expr_subst substU substV n e = e' ->
+      forall _tvs tus tvs tus' tvs'
+             (R : exprT tus tvs (exprT tus' tvs' Prop))
+             (H_substU : forall u t get,
+                 nth_error_get_hlist_nth typD tus u = Some (@existT _ _ t get) ->
+                 match substU u with
+                   | Some eU =>
+                     exists eUD,
+                     exprD' tus' tvs' eU t = Some eUD /\
+                     forall us vs us' vs',
+                       R us vs us' vs' -> get us = eUD us' vs'
+                   | None =>
+                     exists get',
+                        nth_error_get_hlist_nth typD tus' u = Some (@existT _ _ t get')
+                     /\ forall us vs us' vs', R us vs us' vs' -> get us = get' us'
+                 end)
+             (H_substV : forall u t get,
+                 nth_error_get_hlist_nth typD tvs u = Some (@existT _ _ t get) ->
+                 match substV u with
+                   | Some eV =>
+                     exists eVD,
+                     exprD' tus' tvs' eV t = Some eVD /\
+                     forall us vs us' vs', R us vs us' vs' -> get vs = eVD us' vs'
+                   | None => exists get',
+                             nth_error_get_hlist_nth typD tvs' u = Some (@existT _ _ t get')
+                             /\ forall us vs us' vs', R us vs us' vs' -> get vs = get' vs'
+                 end),
+      forall t eD,
+        length _tvs = n ->
+        exprD' tus (_tvs ++ tvs) e t = Some eD ->
+        exists eD',
+          exprD' tus' (_tvs ++ tvs') e' t = Some eD' /\
+          forall us vs us' vs' _vs, R us vs us' vs' ->
+                 eD us (HList.hlist_app _vs vs) = eD' us' (HList.hlist_app _vs vs').
+  Proof.
+    intros.
+    eapply (@expr_subst_sound_ho) in H1; eauto with typeclass_instances.
+    2: instantiate (1 := fun P => forall us vs us' vs', R us vs us' vs' -> P us vs us' vs').
+    { forward_reason.
+      eexists; split; eauto. }
+    { constructor.
+      { intros. eauto. }
+      { intros. eauto. } }
+    eauto. eauto.
+  Qed.
+
+  Corollary mentionsAny_complete_false
+  : forall pu pv e,
+      mentionsAny pu pv e = false <->
+      (forall u, mentionsU u e = true -> pu u = false) /\
+      (forall v, mentionsV v e = true -> pv v = false).
+  Proof.
+    intros.
+    consider (mentionsAny pu pv e); intros; split; auto; intros; try congruence.
+    * eapply mentionsAny_complete in H. destruct H.
+      forward_reason. eauto.
+      forward_reason. eauto.
+    * destruct (mentionsAny_complete pu pv e).
+      clear H1.
+      split; intros.
+      + consider (pu u); auto; intros.
+        exfalso.
+        rewrite H2 in H; try congruence; eauto.
+      + consider (pv v); auto; intros.
+        exfalso.
+        rewrite H2 in H; try congruence; eauto.
+  Qed.
 
 End Expr.
 
-Arguments Safe_expr {_ _ _ Expr} _ _ _ _ : rename.
+(* Arguments Safe_expr {_ _ _ Expr} _ _ _ _ : rename. *)
 Arguments exprD' {_ _ _ Expr} _ _ _ _ : rename.
 Arguments exprD {_ _ _ Expr} _ _ _ _ : rename.
 Arguments exprT {_ RType} _ _ _ : rename.
@@ -344,6 +672,7 @@ Arguments exprT_Inj {_ _} _ _ {_} _ _ _ : rename.
 Arguments exprT_UseU {_ _} tus tvs n : rename.
 Arguments exprT_UseV {_ _} tus tvs n : rename.
 Arguments RexprT {typ RType} tus tvs {_} _ _ _ : rename.
+Arguments mentionsAny {typ RType expr Expr} _ _ _ : rename.
 
 Export MirrorCore.TypesI.
 Export MirrorCore.EnvI.
