theories/Lambda/ExprLift.v
@@ -4,10 +4,11 @@ Require Import ExtLib.Data.HList.
 Require Import ExtLib.Data.Option.
 Require Import ExtLib.Data.Eq.
 Require Import ExtLib.Tactics.
+Require Import MirrorCore.TypesI.
+Require Import MirrorCore.SymI.
 Require Import MirrorCore.Util.Forwardy.
-Require Import MirrorCore.Lambda.ExprD.
 Require Import MirrorCore.Lambda.ExprCore.
-Require Import MirrorCore.Lambda.ExprTac.
+Require Import MirrorCore.Lambda.ExprD.
 
 Set Implicit Arguments.
 Set Strict Implicit.
@@ -39,17 +40,6 @@ Section raw_types.
         App (lift skip _by a) (lift skip _by b)
       | Abs t a =>
         Abs t (lift (S skip) _by a)
-    end.
-
-  Fixpoint vars_to_uvars (skip add : nat) (e : expr typ func) : expr typ func :=
-    match e with
-      | Var v =>
-        if v ?[ lt ] skip then Var v
-        else UVar (v - skip + add)
-      | UVar _
-      | Inj _ => e
-      | App l r => App (vars_to_uvars skip add l) (vars_to_uvars skip add r)
-      | Abs t e => Abs t (vars_to_uvars (S skip) add e)
     end.
 
 End raw_types.
@@ -263,148 +253,5 @@ Section types.
         intros. eapply (IHe us (Hcons x1 vs)). }
       { rewrite H0 in *. congruence. } }
   Qed.
-
-  Theorem vars_to_uvars_typeof_expr
-  : forall tus e tvs tvs' t,
-      typeof_expr tus (tvs ++ tvs') e = Some t ->
-      typeof_expr (tus ++ tvs') tvs (vars_to_uvars (length tvs) (length tus) e)
-      = Some t.
-  Proof.
-    induction e; simpl; intros; auto.
-    { consider (v ?[ lt ] length tvs); intros.
-      { simpl. rewrite ListNth.nth_error_app_L in H; auto. }
-      { simpl. rewrite ListNth.nth_error_app_R in H; auto. 2: omega.
-        rewrite ListNth.nth_error_app_R; try omega.
-        replace (v - length tvs + length tus - length tus) with (v - length tvs)
-          by omega.
-        auto. } }
-    { forward. erewrite IHe1; eauto. erewrite IHe2; eauto. }
-    { forward. eapply (IHe (t :: tvs) tvs') in H.
-      simpl in *.
-      rewrite H in *. auto. }
-    { apply ListNth.nth_error_weaken; auto. }
-  Qed.
-
-  Lemma nth_error_get_hlist_nth_rwR
-  : forall {T} (F : T -> _) tus tvs' n,
-      n >= length tus ->
-      match nth_error_get_hlist_nth F tvs' (n - length tus) with
-        | None => True
-        | Some (existT t v) =>
-          exists val,
-          nth_error_get_hlist_nth F (tus ++ tvs') n = Some (@existT _ _ t val) /\
-          forall a b,
-            v a = val (hlist_app b a)
-      end.
-  Proof.
-    clear. intros.
-    forward. subst.
-    consider (nth_error_get_hlist_nth F (tus ++ tvs') n).
-    { intros.
-      eapply nth_error_get_hlist_nth_appR in H; eauto.
-      destruct s. simpl in *. rewrite H1 in *.
-      destruct H as [ ? [ ? ? ] ]. inv_all; subst.
-      eexists; split; eauto. }
-    { intros.
-      exfalso.
-      eapply nth_error_get_hlist_nth_Some in H1.
-      eapply nth_error_get_hlist_nth_None in H0.
-      forward_reason. simpl in *.
-      eapply ListNth.nth_error_length_ge in H0.
-      clear H1. eapply ListNth.nth_error_length_lt in x0.
-      rewrite app_length in H0. omega. }
-  Qed.
-
-  Definition lem_vars_to_uvars_exprD' : Prop :=
-    forall (tus : tenv typ) (e : _) (tvs : list typ)
-         (t : typ) (tvs' : list typ)
-         (val : hlist typD tus ->
-                hlist typD (tvs ++ tvs') -> typD t),
-    exprD' tus (tvs ++ tvs') t e = Some val ->
-    exists
-      val' : hlist typD (tus ++ tvs') ->
-             hlist typD tvs -> typD t,
-      exprD' (tus ++ tvs') tvs t (vars_to_uvars (length tvs) (length tus) e) = Some val' /\
-      (forall (us : hlist typD tus)
-              (vs' : hlist typD tvs') (vs : hlist typD tvs),
-         val us (hlist_app vs vs') = val' (hlist_app us vs') vs).
-
-  Theorem vars_to_uvars_exprD' : lem_vars_to_uvars_exprD'.
-  Proof.
-    red.
-    induction e; simpl; intros.
-    { revert H; consider (v ?[ lt ] length tvs);
-      autorewrite with exprD_rw; simpl; intros; forwardy.
-      { inv_all; subst.
-        eapply nth_error_get_hlist_nth_appL in H.
-        forward_reason. rewrite H2.
-        rewrite H in H0. inv_all; subst.
-        simpl in *. change_rewrite H1.
-        eexists; split; try reflexivity.
-        simpl. intros. f_equal. apply H3. }
-      { inv_all; subst.
-        eapply nth_error_get_hlist_nth_appR in H0.
-        2: omega.
-        simpl in *.
-        forward_reason.
-        assert (v - length tvs + length tus >= length tus) by omega.
-        eapply nth_error_get_hlist_nth_rwR with (F := typD) in H3.
-        revert H3.
-        instantiate (1 := tvs').
-        cutrewrite (v - length tvs + length tus - length tus = v - length tvs); [ | omega ].
-        change_rewrite H0.
-        intros; forward_reason.
-        change_rewrite H3.
-        change_rewrite H1.
-        eexists; split; try reflexivity.
-        simpl. intros. f_equal. rewrite H2. eapply H4. } }
-    { revert H; autorewrite with exprD_rw; simpl.
-      intros. destruct (funcAs f t); try congruence.
-      eexists; split; try reflexivity.
-      simpl. inv_all; subst. reflexivity. }
-    { revert H. autorewrite with exprD_rw; simpl; intros.
-      forwardy; inv_all; subst.
-      eapply vars_to_uvars_typeof_expr in H.
-      change_rewrite H.
-      eapply IHe1 in H0.
-      eapply IHe2 in H1.
-      forward_reason.
-      Cases.rewrite_all_goal.
-      eexists; split; try reflexivity.
-      intros.
-      unfold exprT_App.
-      autorewrite with eq_rw.
-      rewrite H2. rewrite H3. reflexivity. }
-    { revert H. autorewrite with exprD_rw; simpl; intros.
-      match goal with
-        | H : typ2_match _ ?Y _ _ = _ |- _ =>
-          arrow_case Y
-      end; try congruence.
-      clear H0.
-      red in x1; subst. unfold Relim in *.
-      autorewrite with eq_rw in *. forwardy.
-      change_rewrite H.
-      destruct y0. eapply IHe with (tvs := x :: tvs) in H1.
-      forward_reason.
-      change_rewrite H1.
-      eexists; split; try reflexivity.
-      inv_all; subst. intros.
-      autorewrite with eq_rw.
-      eapply match_eq_match_eq with (F := fun x => x).
-      eapply FunctionalExtensionality.functional_extensionality.
-      intros. specialize (H3 us vs' (Hcons x2 vs)).
-      apply H3. }
-    { revert H. autorewrite with exprD_rw; simpl; intros.
-      forwardy. inv_all; subst.
-      eapply nth_error_get_hlist_nth_weaken in H.
-      simpl in *. forward_reason.
-      rewrite H. change_rewrite H0.
-      eexists; split; try reflexivity.
-      simpl. intros. f_equal. apply H1. }
-  Qed.
-
-  Theorem vars_to_uvars_spec_vars_to_uvars
-  : @VariablesI.vars_to_uvars_spec _ _ _ Expr_expr vars_to_uvars.
-  Proof. apply vars_to_uvars_exprD'. Qed.
 
 End types.
