theories/Lambda/Expr.v
@@ -1,4 +1,261 @@
+Require Import Coq.Classes.Morphisms.
+Require Import Coq.Bool.Bool.
+Require Import ExtLib.Core.RelDec.
+Require Import ExtLib.Tactics.
+Require Import MirrorCore.ExprI.
 Require Export MirrorCore.Lambda.ExprCore.
 Require Export MirrorCore.Lambda.ExprD.
 Require Export MirrorCore.Lambda.ExprLift.
 Require Export MirrorCore.Lambda.ExprSubst.
+
+Section expr.
+  Variable typ : Type.
+  Variable func : Type.
+  Variable RType_typ : RType typ.
+  Variable Typ2_Fun : Typ2 _ Fun.
+  Context {RSym_func : RSym func}.
+
+  (** Reasoning principles **)
+  Context {RTypeOk_typD : RTypeOk}.
+  Context {Typ2Ok_Fun : Typ2Ok Typ2_Fun}.
+  Context {RSymOk_func : RSymOk RSym_func}.
+
+
+  Lemma Proper_mentionsAny
+  : Proper ((@eq uvar ==> @eq bool) ==>
+            (@eq var ==> @eq bool) ==>
+            @eq (expr typ func) ==> @eq bool) mentionsAny.
+  Proof.
+    repeat red. intros; subst.
+    revert x0 y0 x y H0 H.
+    induction y1; simpl; intros; auto.
+    { erewrite IHy1_1; eauto. erewrite IHy1_2; eauto. }
+    { eapply IHy1; eauto.
+      red. intros; subst. destruct y2; eauto. }
+  Qed.
+
+  Lemma mentionsU_ind u
+  : forall (P : expr typ func -> bool -> Prop),
+      (forall v, P (Var v) false) ->
+      (forall s, P (Inj s) false) ->
+      (forall u', P (UVar u') (u ?[ eq ] u')) ->
+      (forall f x rf rx (IHf : P f rf) (IHx : P x rx), P (App f x) (rf || rx)) ->
+      (forall t x rx (IHx : P x rx), P (Abs t x) rx) ->
+      forall e, P e (_mentionsU u e).
+  Proof.
+    assert (forall x, (fun _ : ExprI.var => false) x = false) by reflexivity.
+    generalize dependent (fun _ : ExprI.var => false).
+    induction e; simpl; intros; eauto.
+  Qed.
+
+  Theorem typeof_expr_strengthenU_single
+  : forall (tus : list typ) (tvs : tenv typ) (e : expr typ func)
+           (t t' : typ),
+      _mentionsU (length tus) e = false ->
+      typeof_expr (tus ++ t :: nil) tvs e = Some t' ->
+      typeof_expr tus tvs e = Some t'.
+  Proof.
+    intros tus tvs e t t' H.
+    revert H tvs t'.
+    eapply (mentionsU_ind (length tus)); simpl; intros; auto.
+    { unfold rel_dec in H; simpl in H.
+      consider (EqNat.beq_nat (length tus) u'); intros; try congruence.
+      generalize (ListNth.nth_error_length_lt _ _ H0).
+      rewrite app_length. simpl. intros.
+      rewrite ListNth.nth_error_app_L in H0; auto.
+      omega. }
+    { forward.
+      eapply orb_false_iff in H.
+      destruct H.
+      erewrite IHf; eauto.
+      erewrite IHx; eauto. }
+    { forward.
+      erewrite IHx; eauto. }
+  Qed.
+
+  Theorem exprD'_strengthenU_single
+  : forall (tus : list typ) (tvs : tenv typ) (e : expr typ func)
+           (t t' : typ)
+           (val : exprT (tus ++ t :: nil) tvs (typD t')),
+      _mentionsU (length tus) e = false ->
+      ExprDsimul.ExprDenote.exprD' (tus ++ t :: nil) tvs t' e = Some val ->
+      exists val' : exprT tus tvs (typD t'),
+        ExprDsimul.ExprDenote.exprD' tus tvs t' e = Some val' /\
+        (forall (us : HList.hlist typD tus)
+                (vs : HList.hlist typD tvs) (u : typD t),
+           val (HList.hlist_app us (HList.Hcons u HList.Hnil)) vs = val' us vs).
+  Proof.
+    intros tus tvs e. simpl. revert tvs.
+    induction e; simpl; intros; autorewrite with exprD_rw in *; simpl in *.
+    { forward. eexists; split; eauto.
+      simpl. intros. inv_all; subst. reflexivity. }
+    { forward. eexists; split; eauto.
+      simpl. intros. inv_all; subst. reflexivity. }
+    { forward. inv_all; subst.
+      specialize (H4 _ _ _ _ eq_refl H1).
+      specialize (IHe2 _ _ _ _ H5 H2).
+      forward_reason.
+      erewrite typeof_expr_strengthenU_single; eauto.
+      rewrite H3; clear H3.
+      rewrite H4; clear H4.
+      eexists; split; eauto.
+      intros.
+      unfold exprT_App.
+      autorewrite with eq_rw.
+      rewrite H6; rewrite H7; reflexivity. }
+    { destruct (typ2_match_case t').
+      { forward_reason.
+        rewrite H1 in *; clear H1.
+        unfold Relim in *.
+        autorewrite with eq_rw in *.
+        forward.
+        eapply IHe in H3; eauto.
+        forward_reason.
+        rewrite H3.
+        eexists; split; eauto.
+        intros.
+        inv_all; subst.
+        autorewrite with eq_rw.
+        Require Import ExtLib.Data.Eq.
+        Require Import FunctionalExtensionality.
+        eapply match_eq_match_eq.
+        eapply match_eq_match_eq with (F := fun x => x).
+        eapply functional_extensionality.
+        eauto. }
+      { rewrite H1 in *. congruence. } }
+    { forward. inv_all; subst.
+      cut (u < length tus); intros.
+      { eapply nth_error_get_hlist_nth_appL in H0.
+        forward_reason.
+        rewrite H0 in H1.
+        inv_all; subst. simpl in *.
+        rewrite H3. rewrite H2.
+        eexists; split; eauto.
+        simpl. intros. rewrite H4. reflexivity. }
+      { eapply nth_error_get_hlist_nth_Some in H1.
+        destruct H1. clear H0.
+        eapply ListNth.nth_error_length_lt in x0.
+        consider (EqNat.beq_nat (length tus) u); try congruence.
+        intros. rewrite app_length in *. simpl in *. omega. } }
+  Qed.
+
+  Theorem typeof_expr_strengthenV_single
+  : forall (tus : list typ) (tvs : tenv typ) (e : expr typ func)
+           (t t' : typ),
+      _mentionsV (length tvs) e = false ->
+      typeof_expr tus (tvs ++ t :: nil) e = Some t' ->
+      typeof_expr tus tvs e = Some t'.
+  Proof.
+    intros tus tvs e t t'.
+    revert tvs t'.
+    induction e; simpl; intros; auto.
+    { eapply RelDec.neg_rel_dec_correct in H.
+      generalize (ListNth.nth_error_length_lt _ _ H0).
+      rewrite app_length. simpl. intros.
+      rewrite ListNth.nth_error_app_L in H0; auto.
+      omega. }
+    { forward.
+      erewrite IHe1; eauto.
+      erewrite IHe2; eauto. }
+    { forward.
+      erewrite IHe; eauto. }
+  Qed.
+
+  Theorem exprD'_strengthenV_single
+  : forall (tus : list typ) (tvs : tenv typ) (e : expr typ func)
+           (t t' : typ)
+           (val : HList.hlist typD tus ->
+                  HList.hlist typD (tvs ++ t :: nil) -> typD t'),
+      _mentionsV (length tvs) e = false ->
+      ExprDsimul.ExprDenote.exprD' tus (tvs ++ t :: nil) t' e = Some val ->
+      exists
+        val' : HList.hlist typD tus ->
+               HList.hlist typD tvs -> typD t',
+        ExprDsimul.ExprDenote.exprD' tus tvs t' e = Some val' /\
+        (forall (us : HList.hlist typD tus)
+                (vs : HList.hlist typD tvs) (u : typD t),
+           val us (HList.hlist_app vs (HList.Hcons u HList.Hnil)) = val' us vs).
+  Proof.
+    intros tus tvs e. simpl. revert tvs.
+    induction e; simpl; intros; autorewrite with exprD_rw in *; simpl in *.
+    { forward. inv_all; subst.
+      cut (v < length tvs); intros.
+      { eapply nth_error_get_hlist_nth_appL in H0.
+        forward_reason.
+        rewrite H0 in H1.
+        inv_all; subst. simpl in *.
+        rewrite H3. rewrite H2.
+        eexists; split; eauto.
+        simpl. intros. rewrite H4. reflexivity. }
+      { eapply nth_error_get_hlist_nth_Some in H1.
+        destruct H1. clear H0.
+        eapply ListNth.nth_error_length_lt in x0.
+        eapply RelDec.neg_rel_dec_correct in H.
+        intros. rewrite app_length in *. simpl in *. omega. } }
+    { forward. eexists; split; eauto.
+      simpl. intros. inv_all; subst. reflexivity. }
+    { forward. inv_all; subst.
+      specialize (IHe1 _ _ _ _ H H1).
+      specialize (IHe2 _ _ _ _ H4 H2).
+      forward_reason.
+      erewrite typeof_expr_strengthenV_single; eauto.
+      rewrite H3; clear H3.
+      rewrite H5; clear H5.
+      eexists; split; eauto.
+      intros.
+      unfold exprT_App.
+      autorewrite with eq_rw.
+      rewrite H6; rewrite H7; reflexivity. }
+    { destruct (typ2_match_case t').
+      { forward_reason.
+        rewrite H1 in *; clear H1.
+        unfold Relim in *.
+        autorewrite with eq_rw in *.
+        forward.
+        eapply (IHe (t :: tvs)) in H3; eauto.
+        forward_reason.
+        rewrite H3.
+        eexists; split; eauto.
+        intros.
+        inv_all; subst.
+        autorewrite with eq_rw.
+        eapply match_eq_match_eq.
+        eapply match_eq_match_eq with (F := fun x => x).
+        eapply functional_extensionality.
+        intros.
+        eapply (H5 us (HList.Hcons (Rcast_val r x3) vs)). }
+      { rewrite H1 in *. congruence. } }
+    { forward. eexists; split; eauto.
+      simpl. intros. inv_all; subst. reflexivity. }
+  Qed.
+
+
+  Instance Expr_expr : Expr _ (expr typ func) :=
+  { exprD' := fun tus tvs e t => ExprDsimul.ExprDenote.exprD' tus tvs t e
+  ; wf_Expr_acc := @wf_expr_acc typ func
+  ; expr_subst := @_subst _ _
+  ; mentionsAny := ExprCore.mentionsAny
+  ; mentionsU := _mentionsU
+  ; mentionsV := _mentionsV
+  }.
+
+  Instance ExprOk_expr : ExprOk Expr_expr :=
+  { exprD'_weaken := _
+  }.
+  { intros. eapply (@ExprFacts.exprD'_weaken _ _ _ _ _ _ _ _ _ _ _).
+    eapply H. }
+  { eapply exprD'_strengthenU_single. }
+  { eapply exprD'_strengthenV_single. }
+  { eapply ExprCore.Proper_mentionsAny. }
+  { intros. eapply mentionsAny_weaken; eauto. }
+  { intros. eapply mentionsAny_factor. }
+  { intros. eapply mentionsAny_complete. }
+  { eapply _mentionsU_mentionsU. }
+  { intros. eapply _mentionsV_mentionsV. }
+  { intros. eapply expr_subst_sound; eauto. eapply H. eapply H1. }
+  { intros; eapply _subst_noop; eauto. }
+  { eapply mentionsU_subst. }
+  { eapply mentionsV_subst. }
+  { eapply Proper_subst. }
+  Qed.
+End expr.
