theories/RTac/Apply.v
@@ -3,8 +3,6 @@ Require Import ExtLib.Tactics.
 Require Import MirrorCore.ExprDAs.
 Require Import MirrorCore.Lemma.
 Require Import MirrorCore.LemmaApply.
-Require Import MirrorCore.InstantiateI.
-Require Import MirrorCore.VariablesI.
 Require Import MirrorCore.UnifyI.
 Require Import MirrorCore.RTac.Core.
 Require Import MirrorCore.RTac.Reduce.
@@ -24,18 +22,12 @@ Section parameterized.
   Context {Typ0_Prop : Typ0 _ Prop}.
   Context {Expr_expr : Expr RType_typ expr}.
   Context {ExprOk_expr : ExprOk Expr_expr}.
-  Context {ExprVar_expr : ExprVar expr}.
-  Context {ExprVarOk_expr : ExprVarOk _}.
   Context {ExprUVar_expr : ExprUVar expr}.
   Context {ExprUVarOk_expr : ExprUVarOk _}.
-  Context {MentionsAny_expr : MentionsAny expr}.
-  Context {MentionsAnyOk_expr : MentionsAnyOk _ _ _}.
 
-  Variable vars_to_uvars : nat -> nat -> expr -> expr.
   Variable exprUnify : forall subst, Subst subst expr -> SubstUpdate subst expr ->
     unifier typ expr subst.
 
-  Variable vars_to_uvars_sound : vars_to_uvars_spec vars_to_uvars.
   Variable exprUnify_sound
   : forall subst S (SO : SubstOk S) SU (SUO : SubstUpdateOk _ SO),
       unify_sound (@exprUnify subst S SU).
@@ -44,7 +36,7 @@ Section parameterized.
   Variable lem : Lemma.lemma typ expr expr.
 
   Definition APPLY : rtac typ expr :=
-    @EAPPLY typ expr _ _ _ _ vars_to_uvars exprUnify lem.
+    @EAPPLY typ expr _ _ _ _ exprUnify lem.
 
   Hypothesis lemD :
     @Lemma.lemmaD typ expr _ _ expr (@exprD'_typ0 _ _ _ _ Prop _)
